code/experimental/ed25519/Hacl.Impl.Ed25519.PointCompress.fst
@@ -11,27 +11,72 @@ let hint8_p = buffer Hacl.UInt8.t
 let hint64_p = buffer Hacl.UInt64.t
 let op_String_Access h b = Hacl.Spec.Endianness.reveal_sbytes (as_seq h b)
 
+open FStar.Mul
+
+private let lemma_distr_4 a b c d e : Lemma (a * (b + c + d + e) == a * b + a * c + a * d + a * e)
+  = ()
+
+
+#reset-options "--max_fuel 0 --z3rlimit 20"
+
+private let lemma_x_mod_2 (a:nat) (b:nat) (c:nat) (d:nat) (e:nat) : 
+  Lemma ((a + pow2 51 * b + pow2 102 * c + pow2 153 * d + pow2 204 * e) % 2 = a % 2)
+  = assert_norm(pow2 51 = 2 * pow2 50);
+    assert_norm(pow2 102 = 2 * pow2 101);
+    assert_norm(pow2 153 = 2 * pow2 152);
+    assert_norm(pow2 204 = 2 * pow2 203);
+    lemma_distr_4 2 (pow2 50 * b) (pow2 101 * c) (pow2 152 * d) (pow2 203 * e);
+    Math.Lemmas.paren_mul_right 2 (pow2 50) b;
+    Math.Lemmas.paren_mul_right 2 (pow2 101) c;
+    Math.Lemmas.paren_mul_right 2 (pow2 152) d;
+    Math.Lemmas.paren_mul_right 2 (pow2 203) e;
+    Math.Lemmas.modulo_addition_lemma a 2 ((pow2 50 * b)+(pow2 101 * c)+(pow2 152 * d)+(pow2 203 * e))
+
+private val x_mod_2:
+  x:felem ->
+  Stack Hacl.UInt64.t
+    (requires (fun h -> live h x /\ red_51 (as_seq h x) /\
+      (let s = as_seq h x in
+       FStar.Mul.(Hacl.UInt64.(v (Seq.index s 0)
+                               + pow2 51 * v (Seq.index s 1)
+                               + pow2 102 * v (Seq.index s 2)
+                               + pow2 153 * v (Seq.index s 3)
+                               + pow2 204 * v (Seq.index s 4) == seval (as_seq h x))))))
+    (ensures (fun h0 z h1 -> h0 == h1 /\ live h0 x /\
+      v z = seval (as_seq h0 x) % 2))
+let x_mod_2 x =
+  let h = ST.get() in
+  lemma_x_mod_2 (v (get h x 0)) (v (get h x 1)) (v (get h x 2)) (v (get h x 3)) (v (get h x 4));
+  let x0 = x.(0ul) in
+  let z  = x0 &^ 1uL in
+  assert_norm(pow2 1 = 2);
+  UInt.logand_mask (v x0) 1;
+  z
+
 
 val point_compress:
-  out:hint64_p{length out = 32} ->
+  out:hint8_p{length out = 32} ->
   p:Hacl.Impl.Ed25519.ExtPoint.point ->
   Stack unit
     (requires (fun h -> live h out /\ live h p))
     (ensures (fun h0 _ h1 -> live h0 out /\ live h0 p /\ 
-      live h1 out /\ modifies_1 out h0 h1(*  /\ *)
-      (* h1.[out] == Spec.point_compress  *)
-      ))
+      live h1 out /\ modifies_1 out h0 h1 /\
+      h1.[out] == Spec.point_compress (Hacl.Impl.Ed25519.ExtPoint.as_point h0 p)
+    ))
 let point_compress out p =
   push_frame();
-  let tmp  = create (Hacl.Cast.uint64_to_sint64 0uL) 10ul in
-  let zinv = Buffer.sub tmp 0ul 5ul in
-  let x    = Buffer.sub tmp 5ul 5ul in
+  let tmp  = create (Hacl.Cast.uint64_to_sint64 0uL) 15ul in
+  let zinv = Buffer.sub tmp 0ul  5ul in
+  let x    = Buffer.sub tmp 5ul  5ul in
+  let out  = Buffer.sub tmp 10ul 5ul in
   let px   = Hacl.Impl.Ed25519.ExtPoint.getx p in
   let py   = Hacl.Impl.Ed25519.ExtPoint.gety p in
   let pz   = Hacl.Impl.Ed25519.ExtPoint.getz p in
-  Hacl.Bignum25519.inverse zinv pz;
+  Hacl.Bignum25519.inverse  zinv pz;
   Hacl.Bignum25519.fmul x   px zinv;
+  Hacl.Bignum25519.reduce x;
   Hacl.Bignum25519.fmul out py zinv;
+  Hacl.Bignum25519.reduce out;
   let b = x.(0ul) &^ 1uL in
   let out4 = out.(4ul) in
   out.(4ul) <- out4 +^ (b <<^ 51ul);
