code/experimental/ed25519/Hacl.Bignum25519.fsti
@@ -175,3 +175,19 @@ val reduce:
                                + pow2 102 * v (Seq.index s 2)
                                + pow2 153 * v (Seq.index s 3)
                                + pow2 204 * v (Seq.index s 4) == seval (as_seq h0 out))))))
+
+val lemma_reveal_red_51: s:seqelem ->
+  Lemma (let open Hacl.UInt64 in
+         v (Seq.index s 0) < pow2 51 /\
+         v (Seq.index s 1) < pow2 51 /\
+         v (Seq.index s 2) < pow2 51 /\
+         v (Seq.index s 3) < pow2 51 /\
+         v (Seq.index s 4) < pow2 51)
+
+val lemma_reveal_seval: s:seqelem ->
+  Lemma (FStar.Mul.(Hacl.UInt64.((v (Seq.index s 0)
+                               + pow2 51 * v (Seq.index s 1)
+                               + pow2 102 * v (Seq.index s 2)
+                               + pow2 153 * v (Seq.index s 3)
+                               + pow2 204 * v (Seq.index s 4)) % (pow2 255 - 19) == seval s)))
+
